proved that eqit_secure commutes with bind, lots of work on weakly compatible closures, and began investigating a way to lift PERs to equivalence relations that preserves properness

theories/Secure/SecureEqEuttHalt.v
@@ -24,7 +24,7 @@ From ITree Require Import
      Events.StateFacts
      Core.Divergence
      Dijkstra.TracesIT
-     Secure.SecureEq
+     Secure.SecureEqHalt
 .
 
 From Paco Require Import paco.
@@ -42,6 +42,22 @@ Ltac unpriv_ind := try apply EqVisUnPrivLInd;
                    try apply EqVisUnPrivRInd;
                    auto; intros.
 
+Ltac unpriv_halt :=
+  match goal with
+  | [  Hemp : empty ?A |- secure_eqitF _ _ _ _ _ _ _ _ (@VisF _ _ _ ?A _ _) _ ] =>
+    try apply  EqVisUnprivHaltLTauR; try apply EqVisUnprivHaltLVisR; auto; intros
+
+  | [  Hemp : empty ?A |- secure_eqitF _ _ _ _ _ _ _ _ _ (@VisF _ _ _ ?A _ _)  ] =>
+    try apply EqVisUnprivHaltRTauL; try apply EqVisUnprivHaltRVisL; auto; intros end.
+
+Ltac contra_size :=
+  match goal with
+  | [ Hemp : empty ?A, Hne : nonempty ?A |- _ ] => inv Hemp; inv Hne; contradiction 
+  | [ Hemp : empty ?A, a :?A |- _] => inv Hemp; contradiction
+  end
+.
+
+
 Lemma tau_eqit_secure : forall E R1 R2 Label priv l RR (t1 : itree E R1) (t2 : itree E R2),
     eqit_secure Label priv RR true true l (Tau t1) t2 -> eqit_secure Label priv RR true true l t1 t2.
 Proof.
@@ -50,6 +66,7 @@ Proof.
   hinduction Hsec before priv; intros;  inv Heqx; pclearbot; try inv CHECK; auto.
   - constructor; auto. pstep_reverse.
   - unpriv_ind. pstep_reverse.
+  - punfold H.
 Qed.
 
 Lemma unpriv_e_eqit_secure : forall E A R1 R2 Label priv l RR (e : E A) (k : A -> itree E R1) 
@@ -62,11 +79,12 @@ Proof.
   intros. punfold H0. red in H0. cbn in *. pfold. red.
   remember (VisF e k) as x. genobs_clear t ot.
   hinduction H0 before l; intros; try inv Heqx; 
-  ITrace.inj_existT; subst; try contradiction;  auto.
+  ITrace.inj_existT; subst; try contradiction; try contra_size; auto.
   - constructor; auto. eapply IHsecure_eqitF; eauto.
   - pclearbot. constructor; auto. pstep_reverse.
   - unpriv_ind. pstep_reverse. pclearbot. apply H.
   - unpriv_ind. eapply H0; eauto.
+  - pclearbot. rewrite itree_eta'. pstep_reverse.
 Qed.
 
 
@@ -129,6 +147,8 @@ Proof.
     + constructor; auto. eapply IHHeutt; eauto.
 Qed.
 
+Definition classic_empty := SecureEqHalt.classic_empty.
+
 (*tomorrow start on the transitivity proof *)
 Lemma eutt_secure_eqit_secure : forall E Label priv l R1 R2 RR (t1 t1': itree E R1) (t2 : itree E R2),
     t1 ≈ t1' -> eqit_secure Label priv RR true true l t1 t2 ->
@@ -153,9 +173,13 @@ Proof.
         do 2 rewrite tau_eutt. auto.
       * assert (leq (priv _ e) l \/ ~ leq (priv _ e) l).
         { apply classic. }
-        destruct H as [SECCHECK | SECCHECK].
+        destruct H as [SECCHECK | SECCHECK]; destruct ( classic_empty X  ).
         ++ pclearbot. rewrite itree_eta' at 1. apply eses_aux1 with (m1 := Tau m1); auto.
            do 2 rewrite tau_eutt. auto.
+        ++ pclearbot. rewrite itree_eta' at 1. apply eses_aux1 with (m1 := Tau m1); auto.
+           do 2 rewrite tau_eutt. auto.
+        ++ unpriv_halt. pclearbot. right. eapply CIH; eauto.
+           apply tau_eqit_secure. pfold. auto.
         ++ pclearbot.
            unpriv_co. pclearbot. right. eapply CIH. apply REL. 
            apply tau_eqit_secure. 
@@ -173,21 +197,39 @@ Proof.
       * constructor; auto. eapply IHHsec; eauto.
       * constructor; auto; intros. right. eapply CIH; try apply REL. pclearbot. apply H.
       * rewrite itree_eta' at 1. unpriv_ind. eapply H0; eauto.
-    + punfold Hsec. red in Hsec. pfold. red.
-      cbn in *. (* if its a Tau or a invisible event we are fine*)
-      destruct (observe t2).
-      * inv Hsec. ITrace.inj_existT. subst. unpriv_ind. rewrite H4. rewrite H4 in H1.
-        eapply eses_aux2; eauto. apply REL.
-      * unpriv_co. right. eapply CIH; try apply REL.
-        eapply unpriv_e_eqit_secure; eauto. apply eqit_secure_sym.
-        apply tau_eqit_secure. apply eqit_secure_sym. pfold. auto.
-      * destruct (classic (leq (priv _ e0) l ) ).
-        -- rewrite itree_eta'. unpriv_ind; auto. 
-           inv Hsec; intros; ITrace.inj_existT; subst; try contradiction. cbn.
-           rewrite H5. rewrite H5 in H2. eapply eses_aux1; eauto. apply REL.
-        -- unpriv_co. right. eapply CIH; try apply REL.
-           do 2 (eapply unpriv_e_eqit_secure; eauto; apply eqit_secure_sym).
-           pfold. auto.
+    + destruct (classic_empty u).
+      * pfold. red. cbn.  punfold Hsec. red in Hsec. cbn in *.
+        destruct (observe t2).
+        -- inv Hsec; contra_size.
+        -- unpriv_halt. right. apply CIH with (t1 := Vis e k1).
+           ++ pfold. constructor. left. auto.
+           ++ inv Hsec; ITrace.inj_existT; subst; try contradiction;  try contra_size. pfold. auto.
+              pclearbot. auto.
+        -- inv Hsec; ITrace.inj_existT; subst; try contradiction; try contra_size.
+           ++ unpriv_halt. right. apply CIH with (t1 := Vis e k1).
+              pfold. constructor. auto. rewrite H1 in H3.
+              pfold. apply H3.
+           ++ pclearbot. unpriv_halt. right. apply CIH with (t1 := Vis e k1).
+              pfold. constructor. auto. apply H2.
+           ++ pclearbot. unpriv_halt. contra_size.
+      * pfold. red. cbn.  punfold Hsec. red in Hsec. cbn in *.
+        destruct (observe t2).
+        ++ rewrite itree_eta' at 1. rewrite itree_eta' in Hsec at 1.
+           eapply eses_aux2; eauto. pfold. constructor. auto.
+        ++ unpriv_co. right. apply CIH with (t1 := k1 a); try apply REL.
+           eapply unpriv_e_eqit_secure; eauto. apply eqit_secure_sym.
+           apply tau_eqit_secure. apply eqit_secure_sym. pfold. auto.
+        ++ destruct (classic (leq (priv _ e0) l )).
+           ** rewrite itree_eta' at 1.
+              eapply eses_aux1 with (m1 := Vis e k1); eauto.
+              pfold. constructor. auto.
+           ** destruct (classic_empty X).
+              --- unpriv_halt. right. eapply CIH; try apply REL.
+                  eapply unpriv_e_eqit_secure; eauto. pfold. auto.
+              --- unpriv_co. right. eapply CIH; try apply REL.
+                  (* eapply unpriv_e_eqit_secure; eauto. *)
+                  do 2 (eapply unpriv_e_eqit_secure; eauto; apply eqit_secure_sym).
+                  pfold. auto.
   - eapply IHHeutt; eauto. pstep_reverse.
     apply tau_eqit_secure. pfold. auto.
 Qed.
@@ -213,6 +255,8 @@ Proof.
       hinduction H2 before b2; intros; inv Heqy; try inv CHECK; eauto.
       * pclearbot. constructor; auto; pstep_reverse.
       * pclearbot. unpriv_ind. pstep_reverse.
+      * pclearbot. punfold H.
+    + pclearbot. punfold H2.
   - inv Heqy. inv H; eauto.
     + pclearbot. unpriv_ind. pstep_reverse.
     + rewrite H0 in H2. unpriv_ind. specialize (H2 a).
@@ -221,47 +265,50 @@ Proof.
       hinduction H2 before b2; intros; inv Heqy; try inv CHECK; eauto.
       * pclearbot. constructor; auto. pstep_reverse.
       * unpriv_ind. pclearbot. pstep_reverse.
+      * pclearbot. punfold H.
+    + pclearbot. punfold H2.
 Qed.
 
 
 Lemma eqit_secure_TauLVisR:
   forall (E : Type -> Type) (R3 : Type) (Label : Preorder) (priv : forall x : Type, E x -> L)
     (l : L) (b1 b2 : bool) (R2 : Type) (RR2 : R2 -> R3 -> Prop),
-    (forall (A : Type) (e : E A), ~ leq (priv A e) l -> nonempty A) ->
     forall (t3 : itree E R2) (X : Type) (e : E X) (k : X -> itree E R3) (a : X),
       (~ leq (priv _ e) l) ->
       eqit_secure Label priv RR2 b1 b2 l (Tau t3) (Vis e k) ->
       eqit_secure Label priv RR2 b1 b2 l t3 (k a).
 Proof.
-  intros E R3 Label priv l b1 b2 R2 RR HEv t3 A e k a He Hsec.
+  intros E R3 Label priv l b1 b2 R2 RR t3 A e k a He Hsec.
   punfold Hsec. red in Hsec. cbn in *. 
   remember (TauF t3) as x. remember (VisF e k) as y.
   hinduction Hsec before b2; intros; try discriminate.
   - inv Heqx. inv CHECK.
     remember (VisF e k) as y. pfold. red. clear IHHsec.
     hinduction Hsec before b2; intros; inv Heqy; ITrace.inj_existT;  subst; 
-    try contradiction; eauto.
+    try contradiction; try contra_size; eauto.
     + constructor; auto. pclearbot. pstep_reverse.
     + unpriv_ind. pclearbot. pstep_reverse.
+    + pclearbot. specialize (H a). punfold H.
   - inv Heqx. inv Heqy. ITrace.inj_existT; subst. pclearbot. apply H.
   - inv Heqx. inv Heqy. ITrace.inj_existT; subst. rewrite H2 in H.
     clear H0. clear H2 t1. remember (TauF t3) as x.
     pfold. red. specialize (H a).
-    hinduction H before b2; intros; inv Heqx; eauto.
+    hinduction H before b2; intros; inv Heqx; try contra_size; eauto.
     + pclearbot. constructor; auto. pstep_reverse.
     + pclearbot. unpriv_ind. pstep_reverse.
+    + pclearbot. punfold H.
+  -  pclearbot. inv Heqx. inv Heqy. ITrace.inj_existT; subst. contra_size.
 Qed.
 
 Lemma eqit_secure_TauRVisL:
   forall (E : Type -> Type) (R3 : Type) (Label : Preorder) (priv : forall x : Type, E x -> L)
     (l : L) (b1 b2 : bool) (R2 : Type) RR2,
-    (forall (A : Type) (e : E A), ~ leq (priv A e) l -> nonempty A) ->
     forall (t3 : itree E R2) (X : Type) (e : E X) (k : X -> itree E R3) (a : X),
       (~ leq (priv _ e) l) ->
       eqit_secure Label priv RR2 b1 b2 l (Vis e k) (Tau t3)->
       eqit_secure Label priv RR2 b1 b2 l (k a) t3.
 Proof.
-  intros E R3 Label priv l b1 b2 R2 RR HEv t3 A e k a He Hsec.
+  intros E R3 Label priv l b1 b2 R2 RR t3 A e k a He Hsec.
   punfold Hsec. red in Hsec. cbn in *.
   remember (TauF t3) as x. remember (VisF e k) as y.
   hinduction Hsec before b2; intros; try discriminate.
@@ -270,12 +317,17 @@ Proof.
     try contradiction; eauto.
     + constructor; auto. pclearbot. pstep_reverse.
     + unpriv_ind. pclearbot. pstep_reverse.
+    + contra_size.
+    + contra_size.
+    + pclearbot. specialize (H a). punfold H.
   - inv Heqx. inv Heqy. ITrace.inj_existT; subst. pclearbot. apply H.
   - inv Heqx. inv Heqy. ITrace.inj_existT; subst. pclearbot. rewrite H2 in H. inv CHECK.
     specialize (H a). pfold. red. remember (TauF t3) as y.
-    hinduction H before b2; intros; inv Heqy; eauto.
+    hinduction H before b2; intros; inv Heqy; try contra_size; eauto.
     + pclearbot. constructor; auto. pstep_reverse.
     + pclearbot. unpriv_ind. pstep_reverse.
+    + pclearbot. punfold H.
+  - inv Heqx. inv Heqy. ITrace.inj_existT; subst. contra_size.
 Qed.
     
 Lemma eqit_secure_VisLR:
@@ -300,16 +352,21 @@ Proof.
     specialize (H a).
     rewrite Heqy in H. clear Heqy. remember (VisF e1 k) as y. 
     hinduction H before l; intros; inv Heqy; ITrace.inj_existT; subst; try contradiction;
-    eauto.
+    try contra_size; eauto.
     + pclearbot. constructor; auto. pstep_reverse.
     + unpriv_ind. pclearbot. pstep_reverse.
+    + pclearbot. specialize (H a0). punfold H.
+
   - inv Heqy.  ITrace.inj_existT; subst. inv CHECK. clear H0.
     rewrite Heqx in H. specialize (H a0).
     remember (VisF e0 k0) as y.
     hinduction H before b1; intros; inv Heqy; ITrace.inj_existT; subst; try contradiction;
-    eauto.
+    try contra_size; eauto.
     + pclearbot. constructor; auto. pstep_reverse.
     + pclearbot. unpriv_ind. pstep_reverse.
+    + pclearbot. specialize (H a). punfold H.
+  - inv Heqx; inv Heqy; ITrace.inj_existT; subst. contra_size.
+  - inv Heqx; inv Heqy; ITrace.inj_existT; subst. contra_size.
 Qed.
 
 
@@ -318,7 +375,6 @@ Lemma eqit_secure_trans_aux1:
     (priv : forall x : Type, E x -> L) (l : L) (b2 : bool) (R2 : Type) 
     (RR1 : R1 -> R2 -> Prop) (RR2 : R2 -> R3 -> Prop) (r : itree E R1 -> itree E R3 -> Prop)
     (r0 : R3) (t4 : itree E R2),
-    (forall A (e : E A), (~ leq (priv _ e) l) -> nonempty A) ->
     secure_eqitF Label priv RR2 true b2 l id
                  (upaco2 (secure_eqit_ Label priv RR2 true b2 l id) bot2) (observe t4) 
                  (RetF r0) ->
@@ -328,7 +384,7 @@ Lemma eqit_secure_trans_aux1:
                    (upaco2 (secure_eqit_ Label priv (rcompose RR1 RR2) true b2 l id) r) 
                    (observe t) (RetF r0).
 Proof.
-  intros E R3 R1 Label priv l b2 R2 RR1 RR2 r r0 t4 Hev Ht23 t H.
+  intros E R3 R1 Label priv l b2 R2 RR1 RR2 r r0 t4 Ht23 t H.
   punfold H. red in H. 
   remember (RetF r0) as x.
   hinduction Ht23 before r; intros; inv Heqx; try inv CHECK; auto.
@@ -340,13 +396,15 @@ Proof.
     hinduction H before r; intros; inv Heqy; try inv CHECK; eauto.
     + pclearbot. constructor; auto. pstep_reverse.
     + pclearbot. unpriv_ind. pstep_reverse.
+    + pclearbot. punfold H.
   - assert (Hne : nonempty A). { eauto. } (* add the condition that lets us assume this*) 
     inv Hne. eapply H0; eauto. Unshelve. all : auto.
     remember (VisF e k1) as y.
     hinduction H1 before r; intros; inv Heqy; try inv CHECK; ITrace.inj_existT; subst; 
-    try contradiction; eauto.
+    try contradiction; try contra_size; eauto.
     + pclearbot. constructor; auto. pstep_reverse.
     + pclearbot. unpriv_ind. pstep_reverse.
+    + pclearbot. rewrite itree_eta' at 1. pstep_reverse.
 Qed.
 
 Lemma eqit_secure_trans_aux2:
@@ -354,7 +412,6 @@ Lemma eqit_secure_trans_aux2:
     (priv : forall x : Type, E x -> L) (l : L) (b2 : bool) (R2 : Type) 
     (RR1 : R1 -> R2 -> Prop) (RR2 : R2 -> R3 -> Prop) (r : itree E R1 -> itree E R3 -> Prop)
     (X : Type) (e0 : E X) (k : X -> itree E R3) (t4 : itree E R2),
-    (forall (A : Type) (e : E A), ~ leq (priv A e) l -> nonempty A) ->
     leq (priv X e0) l ->
     secure_eqitF Label priv RR2 true b2 l id
                  (upaco2 (secure_eqit_ Label priv RR2 true b2 l id) bot2) (observe t4) 
@@ -368,7 +425,7 @@ Lemma eqit_secure_trans_aux2:
                    (upaco2 (secure_eqit_ Label priv (rcompose RR1 RR2) true b2 l id) r) 
                    (observe t) (VisF e0 k).
 Proof.
-  intros E R3 R1 Label priv l b2 R2 RR1 RR2 r X e0 k t4 Hev He0 Ht23 CIH0 t Ht.
+  intros E R3 R1 Label priv l b2 R2 RR1 RR2 r X e0 k t4 He0 Ht23 CIH0 t Ht.
   punfold Ht. red in Ht. remember (VisF e0 k) as x.
   hinduction Ht23 before r; intros; inv Heqx; try inv CHECK;
   ITrace.inj_existT; subst; try contradiction; eauto.
@@ -376,6 +433,7 @@ Proof.
     hinduction Ht before r; intros; inv Heqy; try inv CHECK; eauto.
     + pclearbot. constructor; auto. pstep_reverse.
     + pclearbot. unpriv_ind. pstep_reverse.
+    + pclearbot. punfold H.
   - pclearbot. remember (VisF e0 k1) as y.
     hinduction Ht before r; intros; inv Heqy; try inv CHECK;
     ITrace.inj_existT; subst; try contradiction; eauto.
@@ -386,20 +444,167 @@ Proof.
     Unshelve. all : auto. clear H0. rewrite H2 in H.
     remember (VisF e k1) as y.
     hinduction Ht before r; intros; inv Heqy; try inv CHECK; ITrace.inj_existT; subst;
-    try contradiction; eauto.
+    try contradiction; try contra_size; eauto.
     + pclearbot. constructor; auto. pstep_reverse.
     + pclearbot. unpriv_ind. pstep_reverse.
+    + pclearbot. rewrite itree_eta' at 1. pstep_reverse.
+    
+Qed.
+
+
+Lemma secret_halt_trans_1 : forall E Label priv l b1 b2 (R1 R2 R3 A : Type) (RR1 : R1 -> R2 -> Prop)
+            (RR2 : R2 -> R3 -> Prop) t1 (e : E A) k t3,
+    (~ leq (priv A e) l ) ->
+    empty A -> 
+    eqit_secure Label priv RR1 b1 b2 l t1 (Vis e k) ->
+    eqit_secure Label priv RR2 b1 b2 l (Vis e k) t3 ->
+    eqit_secure Label priv (rcompose RR1 RR2) b1 b2 l t1 t3.
+Proof. 
+  intros E Label priv l b1 b2 R1 R2 R3 A RR1 RR2 t1 e k t3 He HA.
+  generalize dependent t3. generalize dependent t1.
+  pcofix CIH. intros t1 t3 Ht1 Ht3.
+  pfold. red. punfold Ht1. red in Ht1. punfold Ht3. red in Ht3.
+  cbn in *. 
+  remember (VisF e k) as x.
+  hinduction Ht1 before r; intros; inv Heqx; ITrace.inj_existT; subst;
+  try contradiction; try contra_size; eauto.
+  - pclearbot. inv Ht3; ITrace.inj_existT; subst; try contradiction; try contra_size.
+    + constructor. right. apply CIH; auto. pfold. auto.
+    + unpriv_co; auto. right. apply CIH; auto. pfold. rewrite H0 in H2. apply H2.
+    + pclearbot. constructor. right. apply CIH; auto.
+    + pclearbot. destruct (classic_empty B).
+      * unpriv_halt. right. apply CIH; auto. pfold. 
+        red. cbn. unpriv_halt.
+      * unpriv_co. right. apply CIH; auto. apply H1.
+    + pclearbot. unpriv_halt. right. apply CIH; auto. pfold.
+      red. cbn. unpriv_halt. contra_size.
+  - pclearbot.  inv Ht3; ITrace.inj_existT; subst; try contradiction; try contra_size.
+    + unpriv_halt. right. apply CIH; auto.
+      * pfold. red. cbn. unpriv_halt.
+      * pfold. auto.
+    + unpriv_halt. right. apply CIH; auto.
+      * pfold. red. cbn. unpriv_halt.
+      * pfold. auto. rewrite H0 in H2. apply H2.
+    + pclearbot. unpriv_halt. right. apply CIH; auto.
+      pfold. red. cbn. unpriv_halt.
+    + pclearbot. unpriv_halt. right. apply CIH.
+      * pfold. red. cbn. unpriv_halt.
+      * apply H1.
+    + unpriv_halt. contra_size.
+  - pclearbot. inv Ht3; ITrace.inj_existT; subst; try contradiction; try contra_size;
+    destruct (classic_empty A0).
+    + unpriv_halt. right. apply CIH; auto.
+      * pfold. red. cbn. unpriv_halt. contra_size.
+      * pfold. auto.
+    + unpriv_co. right. apply CIH; auto; try apply H.
+      pfold. auto.
+    + unpriv_halt. right. apply CIH; auto.
+      * pfold. red. cbn. unpriv_halt. contra_size.
+      * pfold. rewrite H0 in H2. apply H2.
+    + unpriv_co. right. apply CIH. apply H. rewrite H0 in H2.
+      pfold. apply H2.
+    + pclearbot. unpriv_halt. right. apply CIH; auto. pfold.
+      red. cbn. unpriv_halt. contra_size.
+    + pclearbot. unpriv_co. right. apply CIH; auto. apply H.
+    + unpriv_halt. pclearbot. right. apply CIH; try apply H1.
+      pfold. red. cbn. unpriv_halt. contra_size.
+    + pclearbot. destruct (classic_empty B).
+      * unpriv_halt. right. apply CIH; auto. apply H.
+        pfold. red. cbn. unpriv_halt.
+      * unpriv_co. right. apply CIH; eauto. apply H. apply H1.
+    + pclearbot. unpriv_halt. contra_size.
+    + pclearbot. unpriv_halt. right. apply CIH; auto. apply H.
+      pfold. red. cbn. unpriv_halt. contra_size.
+Qed.
+
+Lemma secret_halt_trans_2 :  forall E Label priv l b1 b2 (R1 R2 R3 A : Type) (RR1 : R1 -> R2 -> Prop)
+            (RR2 : R2 -> R3 -> Prop) (e : E A) k t2 t3,
+    (~ leq (priv A e) l ) ->
+    empty A -> 
+    eqit_secure Label priv RR1 b1 b2 l (Vis e k) t2 ->
+    eqit_secure Label priv RR2 b1 b2 l t2 t3 ->
+    eqit_secure Label priv (rcompose RR1 RR2) b1 b2 l (Vis e k) t3.
+Proof. 
+  intros E Label priv l b1 b2 R1 R2 R3 A RR1 RR2 e k t2 t3 He HA.
+  generalize dependent t3. generalize dependent t2.
+  pcofix CIH. intros t2 t3 Ht2 Ht23. pfold.
+  red. cbn. punfold Ht2. punfold Ht23. red in Ht2. red in Ht23.
+  cbn in *. 
+  hinduction Ht23 before r; intros; eauto.
+  - inv Ht2. ITrace.inj_existT; subst. contra_size.
+  - unpriv_halt. right. pclearbot. eapply CIH; eauto.
+    inv Ht2; ITrace.inj_existT; subst; try contra_size; try contradiction; pclearbot;  eauto.
+    pfold. auto.
+  - eapply IHHt23; eauto.
+    inv Ht2; ITrace.inj_existT; subst; try contra_size; try contradiction; pclearbot; eauto.
+    punfold H0.
+  - pclearbot.
+    inv Ht2; ITrace.inj_existT; subst; try contra_size; try contradiction; pclearbot; eauto.
+  - unpriv_halt. pclearbot.  inv SIZECHECK. right. eapply CIH; try apply H. 
+    Unshelve. all : auto.
+    inv Ht2; ITrace.inj_existT; subst; try contra_size; try contradiction; pclearbot; eauto.
+    + pfold. apply H2.
+    + apply H1.
+  - pclearbot. unpriv_halt. right. eapply CIH; try apply H.
+    inv Ht2; ITrace.inj_existT; subst; try contra_size; try contradiction; pclearbot; eauto.
+    pfold. auto.
+  - pclearbot. unpriv_halt. inv SIZECHECK1. inv SIZECHECK2. right. eapply CIH; try apply H.
+    Unshelve. all : auto.
+    inv Ht2; ITrace.inj_existT; subst; try contra_size; try contradiction; pclearbot; eauto.
+    + pfold. apply H2.
+    + apply H1.
+  - inv SIZECHECK.  eapply H0; eauto. Unshelve. all : auto.
+    inv Ht2; ITrace.inj_existT; subst; try contra_size; try contradiction; pclearbot; eauto.
+    rewrite itree_eta' at 1. pstep_reverse.
+  - unpriv_halt. right. eapply CIH; eauto. pfold. apply Ht2.
+    pfold. apply H.
+  - pclearbot. unpriv_halt. right. eapply CIH; eauto. pfold. auto.
+  - unpriv_halt. contra_size.
+  - unpriv_halt. right. pclearbot. eapply CIH with (t2 := Vis e1 k1); eauto.
+    + pfold. auto.
+    + apply H.
+  - unpriv_halt. contra_size.
+Qed.
+
+Lemma eqit_secure_RR_imp : forall E b1 b2 R1 R2 (RR1 RR2 : R1 -> R2 -> Prop) Label priv l 
+                (t1 : itree E R1) (t2 : itree E R2),
+    RR1 <2= RR2 ->
+    eqit_secure Label priv RR1 b1 b2 l t1 t2 ->
+    eqit_secure Label priv RR2 b1 b2 l t1 t2.
+Proof.
+  intros. generalize dependent t2. revert t1.
+  pcofix CIH. intros t1 t2 Ht12. pfold. red.
+  punfold Ht12. red in Ht12.
+  hinduction Ht12 before r; intros; eauto;
+  try (pclearbot; constructor; auto; right; eapply CIH; eauto; fail);
+  try (pclearbot; unpriv_co; right; eapply CIH; eauto; apply H0; fail).
+  pclearbot. constructor; auto. right. eapply CIH; eauto. apply H0.
+  - pclearbot. unpriv_halt. right. eapply CIH; eauto. apply H0.
+  - pclearbot. unpriv_halt. right. eapply CIH; eauto. apply H0.
+Qed.
+
+Lemma secret_halt_trans_3 :  forall E Label priv l b1 b2 (R1 R2 R3 A : Type) (RR1 : R1 -> R2 -> Prop)
+            (RR2 : R2 -> R3 -> Prop)  t1 t2 (e : E A) k,
+    (~ leq (priv A e) l ) ->
+    empty A -> 
+    eqit_secure Label priv RR1 b1 b2 l t1 t2 ->
+    eqit_secure Label priv RR2 b1 b2 l t2 (Vis e k) ->
+    eqit_secure Label priv (rcompose RR1 RR2) b1 b2 l t1 (Vis e k).
+Proof. 
+  intros. apply eqit_secure_sym in H1. apply eqit_secure_sym in H2.
+  apply eqit_secure_sym. eapply secret_halt_trans_2 in H1; eauto.
+  eapply eqit_secure_RR_imp; eauto.
+  intros. inv PR. econstructor; eauto.
 Qed.
 
 Lemma eqit_secure_trans : forall E Label priv l b1 b2 (R1 R2 R3 : Type) (RR1 : R1 -> R2 -> Prop)
             (RR2 : R2 -> R3 -> Prop) (t1 : itree E R1) (t2 : itree E R2) (t3 : itree E R3),
-    (forall A (e : E A), (~ leq (priv _ e) l) -> nonempty A) ->
     eqit_secure Label priv RR1 b1 b2 l t1 t2 ->
     eqit_secure Label priv RR2 b1 b2 l t2 t3 ->
     eqit_secure Label priv (rcompose RR1 RR2) b1 b2 l t1 t3.
 Proof. 
-  intros E Label priv l b1 b2 R1 R2 R3 RR1 RR2 t1 t2 t3 Hev.
-  revert t1 t2 t3. pcofix CIH0. intros t1 t2 t3 Ht12 Ht23.
+  intros E Label priv l b1 b2 R1 R2 R3 RR1 RR2.
+  pcofix CIH0. intros t1 t2 t3 Ht12 Ht23.
   punfold Ht12. red in Ht12. punfold Ht23. red in Ht23. pfold. red.
   hinduction Ht12 before r; intros; try inv CHECK; auto.
   - remember (RetF r2) as x.
@@ -422,14 +627,22 @@ Proof.
       * destruct (classic (leq (priv _ e) l ) ).
         -- inv Ht23; ITrace.inj_existT; subst; try contradiction; try inv CHECK.
            constructor; auto. eapply eqit_secure_trans_aux2; eauto.
-        -- unpriv_co. right. eapply CIH0; eauto.
-           assert (eqit_secure Label priv RR2 b1 b2 l (Tau t3) (Vis e k)).
-           pfold. auto. eapply eqit_secure_TauLVisR; eauto.
+        -- destruct (classic_empty X).
+           ++ rewrite itree_eta'. rewrite itree_eta' at 1.
+              pstep_reverse.
+              eapply paco2_mon with (r := bot2); intros; try contradiction.
+              eapply secret_halt_trans_3 with (t2 := Tau t3); eauto.
+              ** pfold. constructor. left. auto.
+              ** pfold. auto.
+           ++ unpriv_co. right. eapply CIH0; eauto.
+              assert (eqit_secure Label priv RR2 b1 b2 l (Tau t3) (Vis e k)).
+              pfold. auto. eapply eqit_secure_TauLVisR; eauto.
   - apply IHHt12; auto.
     remember (TauF t0) as y. 
     hinduction Ht23 before r; intros; inv Heqy; try inv CHECK; eauto.
     + pclearbot. constructor; auto. pstep_reverse.
     + pclearbot. unpriv_ind. pstep_reverse.
+    + pclearbot. punfold H.
   - pclearbot. remember (VisF e k2) as x.
     hinduction Ht23 before r; intros; inv Heqx; try inv CHECK; ITrace.inj_existT; subst; 
     try contradiction; eauto.
@@ -450,19 +663,27 @@ Proof.
         hinduction Ht23 before r; intros; inv Heqy; try inv CHECK; eauto.
         -- pclearbot. constructor; auto. pstep_reverse.
         -- pclearbot. unpriv_ind. pstep_reverse.
+        -- pclearbot. punfold H.
       * destruct (classic (leq (priv _ e0) l ) ).
         -- rewrite itree_eta'. unpriv_ind. cbn.
            clear IHHt23. remember (k1 a) as t. specialize (H a). setoid_rewrite <- Heqt in H.
            clear Heqt a k1. eapply eqit_secure_trans_aux2; eauto.
-        -- unpriv_co. right. eapply CIH0. apply H.
-           clear IHHt23. pstep. red. remember (VisF e0 k) as y.
-           hinduction Ht23 before r; intros; inv Heqy; try inv CHECK; 
-           ITrace.inj_existT; subst; try contradiction; eauto.
-           ++ pclearbot. constructor; auto. pstep_reverse.
-           ++ unpriv_ind. pclearbot. pstep_reverse.
+        -- destruct (classic_empty X).
+           ++ rewrite itree_eta'. unpriv_ind.
+              pstep_reverse. apply paco2_mon with (r := bot2); intros; try contradiction.
+              eapply secret_halt_trans_3; eauto. apply H.
+              pfold. auto.
+           ++ unpriv_co. right. eapply CIH0. apply H.
+              clear IHHt23. pstep. red. remember (VisF e0 k) as y.
+              hinduction Ht23 before r; intros; inv Heqy; try inv CHECK; 
+                ITrace.inj_existT; subst; try contradiction; try contra_size;  eauto.
+              ** pclearbot. constructor; auto. pstep_reverse.
+              ** unpriv_ind. pclearbot. pstep_reverse.
+              ** pclearbot. rewrite itree_eta' at 1. pstep_reverse.
     + constructor; auto. eapply IHHt23; eauto.
     + pclearbot. unpriv_co. right. eapply CIH0; try apply H0. apply H.
     + rewrite itree_eta' at 1. unpriv_ind. eapply H0; eauto.
+    + unpriv_halt. right. pclearbot. eapply CIH0; eauto. apply H0.
   - pclearbot. 
     genobs_clear t3 ot3. 
     assert (Hne : nonempty A); eauto. inv Hne.
@@ -470,27 +691,35 @@ Proof.
     { destruct ot3; eauto; right; intros; discriminate. }
     destruct H0 as [ [t4 Ht3] | Ht3].
     + subst. constructor. right. eapply CIH0; try apply H.
+      Unshelve. all: auto.
       eapply eqit_secure_TauRVisL; eauto. pfold. auto.
        (* should be fine but new lemma, also shelved goal *)
     + 
       destruct ot3; try (exfalso; eapply Ht4;  eauto; fail  ).
       * inv Ht23; inv CHECK. ITrace.inj_existT. subst. clear CIH0.
         constructor; auto. rewrite H4. eapply eqit_secure_trans_aux1; eauto.
-        rewrite <- H4. apply H1. (* shelved goal*)
+        rewrite <- H4. apply H1. Unshelve. auto. (* shelved goal*)
       * constructor. right. eapply CIH0; try apply H.
         eapply eqit_secure_TauRVisL; eauto. pfold. auto.
         (* same goal as last admit *)
       * destruct (classic (leq (priv _ e0) l ) ).
         -- inv Ht23; try inv CHECK; ITrace.inj_existT; subst; try contradiction.
            constructor; auto. rewrite H5. eapply eqit_secure_trans_aux2; eauto.
-           rewrite <- H5. apply H2.
-        -- unpriv_co. right. eapply CIH0; try apply H. 
-           Unshelve. all : auto.
-           assert (eqit_secure Label priv RR2 b1 b2 l (Vis e k2) (Vis e0 k) ).
-           pfold. auto. eapply eqit_secure_VisLR; eauto.
+           rewrite <- H5. apply H2. Unshelve. all : auto.
+        -- destruct (classic_empty X).
+           ++ rewrite itree_eta'. rewrite itree_eta' at 1. pstep_reverse.
+              eapply paco2_mon with (r := bot2); intros; try contradiction.
+              eapply secret_halt_trans_3 with (t2 := Vis e k2); eauto.
+              ** pfold. red. cbn. unpriv_co.
+              ** pfold. auto.
+           ++ unpriv_co. right. eapply CIH0; try apply H. 
+              Unshelve. all : auto.
+              assert (eqit_secure Label priv RR2 b1 b2 l (Vis e k2) (Vis e0 k) ).
+              pfold. auto. eapply eqit_secure_VisLR; eauto.
   - pclearbot. remember (VisF e2 k2) as x.
     (* maybe need to separate the inductive and coinductive progress cases? *)
     hinduction Ht23 before r; intros; inv Heqx; try inv CHECK; try contradiction; 
+    try contra_size;
     ITrace.inj_existT; subst; auto.
     + constructor; auto. eapply IHHt23; eauto.
     + pclearbot. unpriv_co. right. eapply CIH0; try apply H0. apply H.
@@ -514,22 +743,29 @@ Proof.
         -- constructor; eauto.
         -- pclearbot. unpriv_ind. pstep_reverse.
         -- unpriv_ind. eapply H0; eauto.
-      * assert (Hne : nonempty B); eauto. inv Hne.  
+        -- pclearbot. rewrite itree_eta' at 1. pstep_reverse.
+      * inv SIZECHECK2.  
         destruct (classic (leq (priv _ e) l ) ).
         -- rewrite itree_eta'. unpriv_ind.
            eapply eqit_secure_trans_aux2; eauto. Unshelve. all : auto.
-        -- unpriv_co. right. eapply CIH0; try apply H1.
-           Unshelve. all : auto.
-           clear H0. pstep. red. remember (VisF e k) as y.
-           specialize (H a). clear Heqot2. genobs (k2 a) ok2.
-           clear Heqok2.
-           hinduction H before r; intros; inv Heqy; try inv CHECK;
-           ITrace.inj_existT; subst; try contradiction; eauto.
-           ++ pclearbot. constructor; auto. pstep_reverse.
-           ++ unpriv_ind. pclearbot. pstep_reverse.
+        -- destruct (classic_empty X).
+           ++ unpriv_halt. right. eapply CIH0; eauto. apply H1.
+              pfold. apply H. Unshelve. auto.
+           ++ unpriv_co. right. eapply CIH0; try apply H1.
+              Unshelve. all : auto.
+              clear H0. pstep. red. remember (VisF e k) as y.
+              specialize (H a). clear Heqot2. genobs (k2 a) ok2.
+              clear Heqok2.
+              hinduction H before r; intros; inv Heqy; try inv CHECK;
+                ITrace.inj_existT; subst; try contradiction; try contra_size;  eauto.
+              ** pclearbot. constructor; auto. pstep_reverse.
+              ** unpriv_ind. pclearbot. pstep_reverse.
+              ** pclearbot. rewrite itree_eta' at 1. pstep_reverse.
     + rewrite itree_eta' at 1. unpriv_ind. eapply H0; eauto.
+    + pclearbot. inv SIZECHECK2. unpriv_halt. right. eapply CIH0; eauto. apply H0.
+      apply H. Unshelve. auto.
   - remember (VisF e k2) as x. hinduction Ht23 before r; intros; inv Heqx; try inv CHECK; 
-    ITrace.inj_existT; subst; try contradiction; auto.
+    ITrace.inj_existT; subst; try contradiction; try contra_size;  auto.
     + constructor; auto. eapply IHHt23; eauto.
     + constructor; auto. pclearbot. assert (Hne : nonempty A0); eauto. inv Hne. eapply H0; eauto.
       pstep_reverse. Unshelve. auto.
@@ -537,28 +773,103 @@ Proof.
       pclearbot. pstep_reverse. Unshelve. auto.
     + assert (Hne : nonempty A0). { eauto. } inv Hne. eauto. Unshelve.  auto.
     + unpriv_ind. eauto.
+    + pclearbot. rewrite itree_eta'. pstep_reverse.
+      apply paco2_mon with (r := bot2); intros; try contradiction.
+      inv SIZECHECK0.
+      eapply secret_halt_trans_3 with (t2 := k0 a); eauto.
+      * pfold. apply H1.
+      * apply H.
+  - pclearbot.
+    remember (TauF t0) as y.
+    hinduction Ht23 before r; intros; inv Heqy; subst; eauto; pclearbot.
+    + unpriv_halt. right. eapply CIH0; eauto.
+    + clear IHHt23. rewrite itree_eta'. rewrite itree_eta' at 1.
+      pstep_reverse. apply paco2_mon with (r := bot2); intros; try contradiction.
+      eapply secret_halt_trans_2; eauto. pfold. auto.
+    + unpriv_halt. right. eapply CIH0; eauto. apply H.
+    + rewrite itree_eta' at 1. unpriv_ind. eapply H0; eauto.
+    + unpriv_halt. contra_size.
+  - pclearbot. 
+    inv Ht23; ITrace.inj_existT; subst; try contra_size; try contradiction;
+    try inv CHECK.
+    + constructor. right. eapply CIH0; eauto. pfold. auto.
+    + unpriv_co. right. eapply CIH0; eauto. rewrite H0 in H2.
+      pfold. apply H2.
+    + pclearbot. constructor. right. eapply CIH0; eauto.
+    + pclearbot. destruct (classic_empty B).
+      * unpriv_halt. right. eapply CIH0; eauto. pfold. red. cbn. unpriv_halt.
+      * unpriv_co. right. eapply CIH0; eauto. apply H1.
+    + pclearbot. unpriv_halt. right. eapply CIH0; eauto.
+      pfold. red. cbn. unpriv_halt. contra_size.
+ - pclearbot. rewrite itree_eta' at 1. pstep_reverse.
+   apply paco2_mon with (r := bot2); intros; try contradiction.
+   eapply secret_halt_trans_2 with (t2 := Vis e2 k2); eauto.
+   + pfold. red. cbn. unpriv_halt.
+   + pfold. auto.
+ - pclearbot. destruct (classic_empty A).
+   + inv Ht23; ITrace.inj_existT; subst; try contradiction; try contra_size; try inv CHECK.
+     * unpriv_halt. right. eapply CIH0 with (t2 := Vis e2 k2); eauto.
+       -- pfold. red. cbn. unpriv_halt. contra_size.
+       -- pfold. auto.
+     * unpriv_halt. right. rewrite H1 in H3. eapply CIH0 with (t2 := Vis e2 k2); eauto.
+       -- pfold. red. cbn. unpriv_halt. contra_size.
+       -- pfold. apply H3.
+     * unpriv_halt. pclearbot. right. eapply CIH0; eauto.
+       pfold. red. cbn. unpriv_halt. contra_size.
+     * unpriv_halt. pclearbot. right. eapply CIH0 with (t2 := Vis e2 k2); eauto.
+       -- pfold. red. cbn. unpriv_halt. contra_size.
+       -- apply H2.
+     * unpriv_halt. contra_size.
+   + destruct (observe t3).
+     * inv Ht23; ITrace.inj_existT; subst; try contra_size; try contradiction.
+     * unpriv_co. right. eapply CIH0; eauto. apply H.
+       inv Ht23; ITrace.inj_existT; subst; try contra_size; try contradiction.
+       pfold. auto. pclearbot. auto.
+     * destruct (classic (leq (priv _ e) l ) ).
+       { inv Ht23; ITrace.inj_existT; subst; try contra_size; try contradiction. }
+       destruct (classic_empty X).
+       -- unpriv_halt. right. eapply CIH0; eauto. apply H. pfold. auto.
+       -- unpriv_co. right. eapply CIH0; eauto. apply H.
+          inv Ht23; ITrace.inj_existT; subst; try contra_size; try contradiction.
+          ++ pfold. apply H5.
+          ++ pclearbot. apply H4.
 Qed.
 
 
-Lemma eqit_secure_RR_imp : forall E b1 b2 R1 R2 (RR1 RR2 : R1 -> R2 -> Prop) Label priv l 
-                (t1 : itree E R1) (t2 : itree E R2),
-    RR1 <2= RR2 ->
-    eqit_secure Label priv RR1 b1 b2 l t1 t2 ->
-    eqit_secure Label priv RR2 b1 b2 l t1 t2.
+Lemma eqit_itree_eqit_secure : forall E Label priv l R1 R2 RR (t1 t1': itree E R1) (t2 : itree E R2),
+    t1 ≅ t1' -> eqit_secure Label priv RR false false l t1 t2 ->
+    eqit_secure Label priv RR false false l t1' t2.
 Proof.
-  intros. generalize dependent t2. revert t1.
-  pcofix CIH. intros t1 t2 Ht12. pfold. red.
-  punfold Ht12. red in Ht12.
-  hinduction Ht12 before r; intros; eauto;
-  try (pclearbot; constructor; auto; right; eapply CIH; eauto; fail);
-  try (pclearbot; unpriv_co; right; eapply CIH; eauto; apply H0; fail).
-  pclearbot. constructor; auto. right. eapply CIH; eauto. apply H0.
+  intros E Label priv l R1 R2 RR. pcofix CIH.
+  intros t1 t1' t2 Heq Hsec. pstep. red.
+  punfold Heq. red in Heq. punfold Hsec. red in Hsec.
+  inv Heq; try inv CHECK.
+  - rewrite <- H0 in Hsec. rewrite itree_eta' at 1. pstep_reverse.
+    eapply paco2_mon with (r := bot2); intros; try contradiction. pfold.
+    red. cbn. remember (RetF r2) as x. clear H H0. 
+    hinduction Hsec before r; intros; inv Heqx; eauto.
+  - pclearbot. genobs t2 ot2.
+    assert ( (exists t3, ot2 = TauF t3) \/ (forall t3, ot2 <> TauF t3) ).
+    { destruct ot2; eauto; right; intros; discriminate. }
+    destruct H1 as [ [t3 Ht2] | Ht2].
+    + subst. rewrite Ht2. rewrite Ht2 in Hsec. constructor.
+      right. eapply CIH; eauto. rewrite <- H0 in Hsec. inv Hsec; try inv CHECK. pclearbot. auto.
+    + destruct ot2; try (exfalso; eapply Ht2;  eauto; fail  ).
+      * rewrite <- H0 in Hsec. inv Hsec; try inv CHECK. 
+      * rewrite <- H0 in Hsec. inv Hsec; ITrace.inj_existT; subst; try inv CHECK.
+        -- pclearbot. unpriv_co. right. eapply CIH; eauto. apply H3.
+        -- pclearbot. unpriv_halt. right. eapply CIH; eauto.
+  - rewrite <- H0 in Hsec. inv Hsec; ITrace.inj_existT; subst; try inv CHECK; try contradiction; try contra_size.
+    + pclearbot. constructor; auto. right. eapply CIH; eauto. apply H2.
+    + pclearbot. unpriv_co. right. eapply CIH; eauto. apply H2.
+    + pclearbot. unpriv_co. right. eapply CIH; eauto. apply H2.
+    + pclearbot. unpriv_halt. right. eapply CIH; eauto. pfold. constructor. left. auto.
+    + pclearbot. unpriv_halt. right. eapply CIH with (t1 := Vis e k1); try apply H2.
+      pfold. constructor. left. auto.
+    + pclearbot. unpriv_halt. right. eapply CIH; eauto. apply H2.
 Qed.
-
-
 
 Lemma eqit_secure_eq_trans : forall E R b1 b2 Label priv l (t1 t2 t3 : itree E R),
-    (forall A (e : E A), (~ leq (priv _ e) l) -> nonempty A) ->
     eqit_secure Label priv eq b1 b2 l t1 t2 ->
     eqit_secure Label priv eq b1 b2 l t2 t3 ->
     eqit_secure Label priv eq b1 b2 l t1 t3.
@@ -568,34 +879,105 @@ Proof.
   eapply eqit_secure_trans; eauto.
 Qed.
 
-Lemma eqit_secure_anything : forall E R1 R2 b (RR : R1 -> R2 -> Prop) Label priv l 
+Lemma eqit_secure_anything : forall E R1 b Label priv l 
                       (t1 : itree E R1) t2,
-    (forall A (e : E A), (~ leq (priv _ e) l) -> nonempty A) ->
     eqit_secure Label priv eq b b l t1 t2 ->
     eqit_secure Label priv eq b b l t1 t1.
 Proof.
-  intros. eapply eqit_secure_eq_trans; eauto.
+  intros.
+  eapply eqit_secure_eq_trans; eauto.
   apply eqit_secure_sym. eapply eqit_secure_RR_imp; eauto.
 Qed.
 
 
-(*
+Global Instance proper_eqit_secure_eqit {E} {R1 R2 : Type} {b} {RR : R1 -> R2 -> Prop} {Label priv l} :
+       Proper (eqit eq b b ==> eqit eq b b ==> iff) (@eqit_secure E R1 R2 Label priv RR b b l).
+Proof.
+  repeat intro. destruct b; split; intros.
+  - eapply eutt_secure_eqit_secure; eauto.
+    apply eqit_secure_sym. eapply eutt_secure_eqit_secure; eauto.
+    apply eqit_secure_sym. auto.
+  - assert (x ≈ y); auto. assert (x0 ≈ y0); auto.
+    symmetry in H2.
+    eapply eutt_secure_eqit_secure; eauto.
+    symmetry in H3. apply eqit_secure_sym.
+    eapply eutt_secure_eqit_secure; eauto.
+    apply eqit_secure_sym. auto.
+  - eapply eqit_itree_eqit_secure; eauto.
+    apply eqit_secure_sym. eapply eqit_itree_eqit_secure; eauto.
+    apply eqit_secure_sym. auto.
+  - assert (x ≅ y); auto. assert (x0 ≅ y0); auto.
+    symmetry in H2. symmetry in H3.
+    eapply eqit_itree_eqit_secure; eauto.
+    apply eqit_secure_sym. eapply eqit_itree_eqit_secure; eauto.
+    apply eqit_secure_sym. auto.
+Qed.
+
+Global Instance proper_eqit_secure_eqit_secure 
+       {E} {b} {R1 R2 : Type} {RR : R1 -> R2 -> Prop} {Label priv l} :
+  Proper (eqit_secure Label priv eq b b l ==> eqit_secure Label priv eq b b l ==> iff) 
+         (@eqit_secure E R1 R2 Label priv RR b b l).
+Proof.
+  repeat intro; split; intros.
+  - eapply eqit_secure_RR_imp with (RR1 := rcompose RR eq); eauto.
+    { intros. inv PR. auto. }
+    eapply eqit_secure_trans; eauto.
+    apply eqit_secure_sym.
+    eapply eqit_secure_RR_imp with (RR1 := rcompose (flip RR) eq); eauto.
+    { intros. inv PR. auto. }
+    eapply eqit_secure_trans; eauto. apply eqit_secure_sym. auto.
+  - assert (eqit_secure Label priv eq b b l y0 x0).
+    { apply eqit_secure_sym. eapply eqit_secure_RR_imp; eauto. }
+    eapply eqit_secure_RR_imp with (RR1 := rcompose RR eq).
+    { intros. inv PR. auto. }
+    eapply eqit_secure_trans; eauto.
+    assert (eqit_secure Label priv eq b b l y x).
+    { apply eqit_secure_sym. eapply eqit_secure_RR_imp; eauto. }
+    eapply eqit_secure_RR_imp with (RR1 := rcompose eq RR).
+    { intros. inv PR. auto. }
+    eapply eqit_secure_trans; eauto.
+Qed.
+
+   (*
+Metatheory goals
 
 
-F : C -> C (monotonic)
+1: eqit_secure lifts PERs to PERs
 
-paco F bot = F (paco F bot)
-
-
-
-t1 ≅ t2
-paco F r t1 t2
+2: interaction with bind
+   eqit_secure RR m1 m2 -> (forall a b, RR a b -> eqit_secure RR' (k1 a) (k2 b)) -> eqit_secure RR' (m1 >>= k1) (m2 >>= k2)
 
 
+3: interaction with iter : (A -> itree E (A + B)) -> A -> itree E B
+   iter body init ≅ Tau (body init >>= (case (iter body) id))
 
-clo (gpaco clo F r g)
-------------------------
-gpaco clo F r g
 
+  RR'' (inl a) (inl b) ->
+  (forall a b, RR a b -> eqit_secure RR'' (body1 a) (body2 b)) -> forall a b, RR a b -> eqit_secure RR' (iter body1 a) (iter body2 b) 
+
+  Prove a itree secure without direct coinduction by mutating it (with valid security preserving rewrites) to a tree with no private events
+
+4: interaction with interp {M : MonadIter} (handler : forall A, E A -> M A) (t : itree E A) : M A
+
+   handler takes secure programs to secure programs -> interp handler takes secure programs to secure programs
+
+   Can we find out the smallest relation that a handler preserves securely automatically
+
+   I have a handwritten relation that I want to be my secure computation comparison, how does it relate to the automatically generated because
+
+   wp post m := fun s => post (m s)
+
+
+5: define ASM with secrecy
+
+6: secure compilation from Imp with secrecy to ASM with secrecy
+
+Definition if_comp : bexp -> com -> asm
+
+while
+  
+
+
+Definition out_RR {E E' R1 R2} Label priv RR l (handler : forall A, E A -> StateT S (itree E') A) : R1 -> R2 -> Prop := 
 
 *)
