theories/Secure/SecureEqBind.v
@@ -1,0 +1,446 @@
+From Coq Require Import
+     Arith.PeanoNat
+     Lists.List
+     Strings.String
+     Morphisms
+     Setoid
+     RelationClasses
+     Logic.Classical_Prop
+     Logic.EqdepFacts
+     Program.Equality
+.
+
+From ExtLib Require Import
+     Data.String
+     Structures.Monad
+     Structures.Traversable
+     Data.List.
+
+From ITree Require Import
+     ITree
+     ITreeFacts
+     Events.MapDefault
+     Events.State
+     Events.StateFacts
+     Core.Divergence
+     Dijkstra.TracesIT
+     Secure.SecureEqHalt
+     Secure.SecureEqEuttHalt
+     Secure.SecureEqWcompat
+.
+
+From Paco Require Import paco.
+
+Import Monads.
+Import MonadNotation.
+Local Open Scope monad_scope.
+
+Section gstep_reverse.
+
+Lemma gpaco2_step_reverse T0 T1 gf clo r rg
+      (MON: monotone2 gf)
+      (WCMP: wcompatible2 gf clo):
+  @gpaco2 T0 T1 gf clo r rg <2= gf (gpaco2 gf clo rg rg).
+Proof.
+  intros.
+  inv WCMP. gunfold PR.
+  induction PR.
+  - destruct IN.
+    + (* need to add constraints that should hold *) admit.
+    + apply wcompat2_wcompat. (* does not seem to hold *) admit.
+  - apply H. (* also don't see why this should hold *) admit.
+  (* gpaco2_intro and gpaco2_dist *) 
+(* apply wcompat2_wcompat.
+
+  apply wcompat2_wcompat. 
+
+
+
+eapply MON with (r := gupaco2 gf clo r); auto.
+  apply wcompat2_wcompat.
+  induction PR.
+  - destruct IN.
+    + admit.
+    + eapply MON with (r := gupaco2 gf clo r).
+      *  apply wcompat2_wcompat. admit.
+         (* what if the clo is strictly increasing *)
+         (* what if the gf is strictly increasing *)
+      * intros. red in PR. auto.
+  - apply wcompat2_wcompat. eapply wcompat2_mon; eauto.
+    intros. apply H in PR. eapply MON; eauto. intros. inv PR0.
+    
+
+      unfold monotone2 in *. admit.
+  -
+  
+
+apply gpaco2_init in PR; [|apply WCMP].
+  _punfold PR; [..|apply gf_mon].
+  eapply gf_mon. apply PR.
+  intros. destruct PR0; [|contradiction]. apply gpaco2_final. apply gf_mon. right. apply H.
+Qed.
+ *) Abort. 
+End gstep_reverse.
+
+
+(*
+
+Inductive
+rclo2 (T0 : Type) (T1 : T0 -> Type) (clo : rel2 T0 T1 -> rel2 T0 T1) 
+(r : rel2 T0 T1) : rel2 T0 T1 :=
+    rclo2_base : forall (x0 : T0) (x1 : T1 x0), r x0 x1 -> rclo2 clo r x0 x1
+  | rclo2_clo' : forall (r' : forall x : T0, T1 x -> Prop) (x0 : T0) (x1 : T1 x0),
+                 (forall (x2 : T0) (x3 : T1 x2), (r' x2 x3 : Prop) -> rclo2 clo r x2 x3 : Prop) ->
+                 clo r' x0 x1 -> rclo2 clo r x0 x1
+
+
+Lemma gpaco2_unfold_bot' gf clo
+      (WCMP: wcompatible2 gf clo):
+  gpaco2 gf clo bot2 bot2 <2= gf (gpaco2 gf clo bot2 bot2).
+Proof.
+  intros. apply gpaco2_init in PR; [|apply WCMP].
+  _punfold PR; [..|apply gf_mon].
+  eapply gf_mon. apply PR.
+  intros. destruct PR0; [|contradiction]. apply gpaco2_final. apply gf_mon. right. apply H.
+Qed.
+*)
+(* try to write a proof that mirrors the gstepreverse thing you want
+   see if, where, something goes wrong come to yannick with that,
+   possibly he or gil or paul would understand
+   do this next week
+*)
+
+(* 
+   Possible ways forward
+   1. try to prove secure_eqit_bind "dumbly" just paco no gpaco
+   2. prove weak compatibility for secure_eqitC
+      2 a. define a secure_bindC closure and prove the relavant relation to secure_eqitC
+   3. find a way to work with gpaco inductive steps
+
+*)
+
+Lemma eqit_bind_shalt_aux1:
+  forall (E : Type -> Type) (S2 S1 R1 R2 : Type) (RR : R1 -> R2 -> Prop)
+    (RS : S1 -> S2 -> Prop) (b1 b2 : bool) (Label : Preorder)
+    (priv : forall A : Type, E A -> L) (l : L) (k1 : R1 -> itree E S1) 
+    (k2 : R2 -> itree E S2) (A : Type) (e : E A) (k0 : A -> itree E R1) 
+    (t2 : itree E R2),
+    ~ leq (priv A e) l ->
+    empty A ->
+    paco2 (secure_eqit_ Label priv RR b1 b2 l id) bot2 (Vis e k0) t2 ->
+    forall (t1 : itree E R1),
+      VisF e k0 = observe t1 ->
+      paco2 (secure_eqit_ Label priv RS b1 b2 l id) bot2 (ITree.bind t1 k1) (ITree.bind t2 k2).
+Proof.
+  intros E S2 S1 R1 R2 RR RS b1 b2 Label priv l k1 k2 A e k0 t2 SECCHECK SIZECHECK H0 t1 Heqot1.
+  pstep. red. unfold ITree.bind at 1, observe at 1. cbn. rewrite <- Heqot1.
+  cbn. rewrite itree_eta' at 1. pstep_reverse.
+  generalize dependent t2. pcofix CIH. intros t2 Ht2.
+  pstep. red. 
+  punfold Ht2. red in Ht2.
+  unfold ITree.bind at 1, observe at 3. cbn in *.
+  inv Ht2; ITrace.inj_existT; subst; try contra_size; try contradiction; try rewrite <- H; cbn;
+  try unpriv_halt; right; eapply CIH;  pclearbot; eauto;
+  try (pfold; rewrite H in H1; apply H1).
+  contra_size.
+Qed.
+
+Lemma eqit_bind_shalt_aux2:
+  forall (E : Type -> Type) (S2 S1 R1 R2 : Type) (RR : R1 -> R2 -> Prop)
+    (RS : S1 -> S2 -> Prop) (b1 b2 : bool) (Label : Preorder)
+    (priv : forall A : Type, E A -> L) (l : L) (k1 : R1 -> itree E S1) 
+    (k2 : R2 -> itree E S2) (A : Type) (e : E A) (k0 : A -> itree E R2) 
+    (t1 : itree E R1) (t2 : itree E R2),
+    ~ leq (priv A e) l ->
+    empty A ->
+    paco2 (secure_eqit_ Label priv RR b1 b2 l id) bot2 t1 (Vis e k0) ->
+    VisF e k0 = observe t2 ->
+    paco2 (secure_eqit_ Label priv RS b1 b2 l id) bot2 (ITree.bind t1 k1) (ITree.bind t2 k2).
+Proof.
+  intros E S2 S1 R1 R2 RR RS b1 b2 Label priv l k1 k2 A e k0 t1 t2 SECCHECK SIZECHECK H0 Heqot1.
+  pstep. red. unfold ITree.bind at 2, observe at 2. cbn. rewrite <- Heqot1.
+  cbn. rewrite itree_eta'. pstep_reverse.
+  generalize dependent t1. pcofix CIH. intros t1 Ht1.
+  pstep. red. 
+  punfold Ht1. red in Ht1.
+  unfold ITree.bind at 1, observe at 1. cbn in *.
+  inv Ht1; ITrace.inj_existT; subst; try contra_size; try contradiction; cbn; 
+  try unpriv_halt; try contra_size; try (right; eapply CIH; pclearbot; eauto).
+  pfold. rewrite H0 in H1. auto. apply H1.
+Qed.
+
+Lemma secure_eqit_bind : forall E R1 R2 S1 S2 (RR : R1 -> R2 -> Prop) (RS : S1 -> S2 -> Prop) 
+                           b1 b2 Label priv l 
+    (t1 : itree E R1) (t2 : itree E R2) (k1 : R1 -> itree E S1) (k2 : R2 -> itree E S2),
+    (forall r1 r2, RR r1 r2 -> eqit_secure Label priv RS b1 b2 l (k1 r1) (k2 r2) ) ->
+    eqit_secure Label priv RR b1 b2 l t1 t2 ->
+    eqit_secure Label priv RS b1 b2 l (ITree.bind t1 k1) (ITree.bind t2 k2).
+Proof.
+  intros. revert H0. revert t1 t2. pcofix CIH. intros t1 t2 Ht12.
+  punfold Ht12. red in Ht12.
+  genobs t1 ot1. genobs t2 ot2.
+  hinduction Ht12 before r; intros; eauto.
+  - pstep. red. unfold ITree.bind, observe. unfold observe in *. cbn.
+    rewrite <- Heqot1. rewrite <- Heqot2. pstep_reverse. eapply paco2_mon with (r := bot2); intros; try contradiction.
+    apply H; auto.
+  - pstep. red. unfold ITree.bind, observe. unfold observe in *. cbn.
+    rewrite <- Heqot1. rewrite <- Heqot2. cbn. constructor. right. eapply CIH. pclearbot.
+    auto.
+  - pstep. red. unfold ITree.bind at 1, observe at 1. cbn.
+    rewrite <- Heqot1. cbn. constructor; auto. pstep_reverse.
+  - pstep. red. unfold ITree.bind at 2, observe at 2. cbn.
+    rewrite <- Heqot2. cbn. constructor; auto. pstep_reverse.
+  - pstep. red. unfold ITree.bind, observe. unfold observe in *. cbn.
+    rewrite <- Heqot1. rewrite <- Heqot2. cbn. pclearbot.
+    constructor; auto. right. eapply CIH; eauto. apply H0.
+  - pstep. red. unfold ITree.bind, observe. unfold observe in *. cbn.
+    rewrite <- Heqot1. rewrite <- Heqot2. cbn. unpriv_co.
+    right. pclearbot. eapply CIH; apply H0.
+  - pstep. red. unfold ITree.bind, observe. unfold observe in *. cbn.
+    rewrite <- Heqot1. rewrite <- Heqot2. cbn. unpriv_co.
+    right. pclearbot. eapply CIH; apply H0.
+  - pstep. red. unfold ITree.bind, observe. unfold observe in *. cbn.
+    rewrite <- Heqot1. rewrite <- Heqot2. cbn. unpriv_co.
+    right. pclearbot. eapply CIH; apply H0.
+  - pstep. red. unfold ITree.bind at 1, observe at 1. cbn.
+    rewrite <- Heqot1. cbn. unpriv_ind. pstep_reverse.
+  - pstep. red. unfold ITree.bind at 2, observe at 2. cbn.
+    rewrite <- Heqot2. cbn. unpriv_ind. pstep_reverse.
+  - pclearbot.
+    eapply paco2_mon with (r := bot2); intros; try contradiction.
+    eapply eqit_bind_shalt_aux1; eauto. pfold. red. rewrite <- Heqot2.
+    cbn. unpriv_halt. left. eauto.
+  - pclearbot.
+    eapply paco2_mon with (r := bot2); intros; try contradiction.
+    eapply eqit_bind_shalt_aux2; eauto. pfold. red. cbn. rewrite <- Heqot1.
+    unpriv_halt. left. eauto.
+  - pclearbot.
+    eapply paco2_mon with (r := bot2); intros; try contradiction.
+    eapply eqit_bind_shalt_aux1 with (A := A); eauto.
+    pfold. red. rewrite <- Heqot2. cbn. unpriv_halt.
+  - pclearbot.
+    eapply paco2_mon with (r := bot2); intros; try contradiction.
+    eapply eqit_bind_shalt_aux2; eauto. pfold. red. cbn. rewrite <- Heqot1.
+    unpriv_halt.
+Qed.
+
+Lemma secure_eqit_iter : forall E A1 A2 B1 B2 (RA : A1 -> A2 -> Prop) (RB : B1 -> B2 -> Prop)
+                           b1 b2 Label priv l 
+                           (body1 : A1 -> itree E (A1 + B1) ) (body2 : A2 -> itree E (A2 + B2) )
+                           (a1 : A1) (a2 : A2),
+    RA a1 a2 -> 
+    (forall a1 a2, RA a1 a2 -> eqit_secure Label priv (HeterogeneousRelations.sum_rel RA RB) b1 b2 l (body1 a1) (body2 a2) ) ->
+    eqit_secure Label priv RB b1 b2 l (ITree.iter body1 a1) (ITree.iter body2 a2).
+Proof.
+  intros. rename H0 into Hbody. generalize dependent a2. revert a1. 
+  (* gcofix CIH. intros. setoid_rewrite unfold_iter.
+  guclo eqit_bind_clo. *)
+
+  (* look into the more general secure_eqitC closure, see if that is weakly compatible, *)
+  pcofix CIH.
+  intros a1 a2 Ha. specialize (Hbody a1 a2 Ha) as Hbodya.
+  punfold Hbodya. red in Hbodya. pfold. red.
+  unfold observe. (* write lemmas for unfolding the observe of iter *) cbn.
+  hinduction Hbodya before r; intros; cbn; auto.
+  - inv H; cbn; eauto.
+  - cbn. pclearbot. constructor. 
+    left. generalize dependent t2. revert t1. pcofix CIH. intros. 
+    
+
+Locate eutt_iter'.
+    (* my choices seem to be nested induction/coinduction or figure out eqit_bind_clo thing *)
+    admit. (* confusing case but probably will come up a lot *)
+  - constructor; auto. right. pclearbot.
+  - cbn. auto. constructor; auto.
+  - cbn. constructor; auto.
+
+    
+    
+    
+
+(*
+(*  eqit_bind' *)
+Lemma secure_eqit_bind : forall E R1 R2 S1 S2 (RR : R1 -> R2 -> Prop) (RS : S1 -> S2 -> Prop) 
+                           b1 b2 Label priv l 
+    (t1 : itree E R1) (t2 : itree E R2) (k1 : R1 -> itree E S1) (k2 : R2 -> itree E S2),
+    (forall r1 r2, RR r1 r2 -> eqit_secure Label priv RS b1 b2 l (k1 r1) (k2 r2) ) ->
+    eqit_secure Label priv RR b1 b2 l t1 t2 ->
+    eqit_secure Label priv RS b1 b2 l (ITree.bind t1 k1) (ITree.bind t2 k2).
+Proof.
+  intros. revert H0. revert t1 t2. ginit.
+  gcofix CIH. intros t1 t2 Ht12. punfold Ht12. red in Ht12.
+  genobs t1 ot1. genobs t2 ot2.
+  hinduction Ht12 before r; intros; eauto.
+  - apply simpobs in Heqot1. setoid_rewrite Heqot1. apply simpobs in Heqot2.
+    setoid_rewrite Heqot2. repeat rewrite bind_ret_l.
+    gfinal. right. eapply paco2_mon with (r := bot2); intros; try contradiction.
+    apply H. auto.
+  - apply simpobs in Heqot1. setoid_rewrite Heqot1. apply simpobs in Heqot2.
+    setoid_rewrite Heqot2. pclearbot. repeat rewrite bind_tau.
+    gstep. constructor. gfinal. left. eapply CIH; eauto.
+  - apply simpobs in Heqot1. rewrite Heqot1. rewrite bind_tau. admit.
+(* gpaco2_intro and gpaco2_dist *) (*
+    apply gpaco2_intro. constructor. left. pfold.
+    constructor; auto. 
+    assert (gpaco2 (secure_eqit_ Label priv RS b1 b2 l id) (eqitC RS b1 b2) bot2 r 
+                   (ITree.bind t1 k1) (ITree.bind t2 k2) ).
+    { eapply IHHt12; eauto. }
+    eapply gpaco2_dist in H0; auto with paco.
+    destruct H0.
+    + punfold H0. red in H0. unfold compose. eapply H0.
+
+pstep_reverse.
+    assert ()
+
+    (* would be nice to have the geutt rewrite rules here *)
+    admit. *)
+  - apply simpobs in Heqot2. rewrite Heqot2. rewrite bind_tau.
+    admit.
+  - apply simpobs in Heqot1. apply simpobs in Heqot2. 
+    rewrite Heqot1. rewrite Heqot2. repeat rewrite bind_vis.
+    gstep. pclearbot. constructor; auto. intros.
+    gfinal. left. eapply CIH; eauto. apply H0.
+  - apply simpobs in Heqot1. apply simpobs in Heqot2. 
+    rewrite Heqot1. rewrite Heqot2. rewrite bind_vis. rewrite bind_tau.
+    pclearbot.
+    gstep. unpriv_co. gfinal. left. eapply CIH; eauto. apply H0.
+  - apply simpobs in Heqot1. apply simpobs in Heqot2. 
+    rewrite Heqot1. rewrite Heqot2. rewrite bind_vis. rewrite bind_tau.
+    pclearbot.
+    gstep. unpriv_co. gfinal. left. eapply CIH; eauto. apply H0.
+  - pclearbot. apply simpobs in Heqot1. apply simpobs in Heqot2. 
+    rewrite Heqot1. rewrite Heqot2. repeat rewrite bind_vis.
+    gstep. unpriv_co. gfinal. left. eapply CIH; eauto. apply H0.
+  - apply simpobs in Heqot1. rewrite Heqot1. rewrite bind_vis.
+
+    gstep. red. cbn. unpriv_ind. 
+        assert (gpaco2 (secure_eqit_ Label priv RS b1 b2 l id) (eqitC RS b1 b2) bot2 r (ITree.bind (k0 a) k1) (ITree.bind t0 k2) ).
+    { eapply H1; eauto. }
+    gunfold H2. 
+    (* getting euttge style rewrites here won't help, because we can only remove
+       private events from well behaved trees, not arbitrary ones,
+       that makes it a weaker reasoning principle than Tau t >= t*)
+    apply gpaco2_intro. constructor. left.
+    pfold. red. red. cbn. unpriv_ind.
+    unfold compose.
+
+    apply gpaco2_dist in H2; auto with paco.
+    destruct H2.
+    + punfold H2. red in H2. eapply secure_eqit_mono; eauto.
+      intros. pclearbot. destruct PR.
+      * constructor. left. (* equivalent to H3 by eta expansion ?*) admit.
+      * induction H3.
+        -- constructor. right. auto.
+        -- eapply rclo2_clo'; eauto.
+    + remember (ITree.bind (k0 a) k1 ) as x.
+      remember (ITree.bind t0 k2) as y.
+      clear Heqx Heqy.
+      induction H2; try contradiction. admit.
+    (* gfinal. right. pfold. red. cbn. unpriv_ind.
+    pstep_reverse. specialize (H1 a CIH (k0 a) t0). *)
+    (*
+    (* gpaco2_step*)
+    gstep. unpriv_ind. 
+
+        assert (gpaco2 (secure_eqit_ Label priv RS b1 b2 l id) (eqitC RS b1 b2) bot2 r (ITree.bind (k0 a) k1) (ITree.bind t0 k2) ).
+    { eapply H1; eauto. }
+    (* write a fold secure_eqit_ ltac *)
+    match goal with 
+      | |- (secure_eqitF ?L ?p ?RR ?b1 ?b2 ?l id) (gpaco2 ?gf' ?clo ?rg ?rg ) (observe ?t1) (observe ?t2) => 
+        enough (secure_eqit_ L p RR b1 b2 l id (gpaco2 gf' clo rg rg) t1 t2  ); eauto end. 
+    (* how does this relate to weak compatibility? *)
+
+    (* shows the structure that I want *)
+      (*  match goal with 
+      | H : gpaco2 ?gf' ?clo ?r ?rg ?t1 ?t2 |- ?gf (gpaco2 ?gf' ?clo ?rg ?rg ) (observe ?t1) (observe ?t2) => idtac gf' end. *)
+    (* gpaco2_unfold is probably where to start *)
+    (* wtf is rclo2 
+       r \2/ (forall r')
+       
+
+     *)
+
+    (* gpaco2 gf clo r rg <2= gf  *)
+    remember (ITree.bind (k0 a) k1 ) as x.
+    remember (ITree.bind t0 k2) as y.
+    clear Heqx Heqy.
+    apply gpaco2_unfold in H2; auto with paco.
+    specialize (eqit_secureC_wcompat_id b1 b2 E S1 S2 RS Label priv l) as Hwcompat.
+    inv Hwcompat. 
+    induction H2; eauto.
+    + destruct IN; try contradiction. 
+      eapply secure_eqit_mono; eauto; intros; eauto with paco.
+      red in PR. eapply gpaco2_mon; eauto. intros. inv PR0; auto; try contradiction.
+      intros. inv PR0; auto. contradiction.
+    + apply wcompat2_wcompat. eapply eqitC_mon; eauto. 
+      intros. apply H2 in PR as H3.
+
+(* *) *)
+    econstructor; try reflexivity.
+    all : intros; try subst; auto.
+    (* go rid of  *)
+    pstep_reverse.
+    induction H2.
+    + destruct IN; try contradiction. 
+      admit.
+    +  inv IN. inv CHECK.
+       specialize (H2 _ _ REL).
+       (* swap in t1' for x0 and x1 for t2'
+          then apply H2 and 
+          this should hold but uggh
+*)
+      (* gpaco2 should be monotonic *)
+      (* gupaco2 should be monotonic *) admit.
+    + inv IN. apply LE in REL.
+ inv H2. 
+    destruct IN; try contradiction.
+    + red in H2. admit.
+    + admit.
+    fold (@secure_eqit_ E R1 R2).
+    eapply gpaco2_clo in H2; eauto.
+    eapply gpaco2_dist in H2; eauto with paco.
+    destruct H2.
+    + punfold H2. admit.
+    + induction H2; try contradiction. 
+
+    Locate gpaco2_unfold_bot.
+    eapply gpaco2_unfold_bot with (clo  := eqitC RS b1 b2) (x0 := ITree.bind (k0 a) k1 ) 
+    (x1 := ITree.bind t0 k2) ; eauto with paco.
+    admit.
+    { constructor; auto with paco.
+      
+
+    { eapply eqit_secureC_wcompat_id.
+
+(* either want something like gstep_reverse or the 
+                          equivalent of geutt rewriting for this functor
+*)
+     enough (gpaco2 (secure_eqit_ Label priv RS b1 b2 l id) (eqitC RS b1 b2) bot2 r
+         (ITree.bind (k0 a) k1) (ITree.bind t0 k2) ).
+    { gunfold H2. Locate Ltac pfold_reverse.  inv H2. destruct IN; try contradiction.
+      - eapply secure_eqit_mono; eauto. intros. eapply gpaco2_gupaco; eauto.
+      -
+      red in H2.
+      eapply secure_eqit_mono; eauto. *)
+(*
+   admit.
+  - apply simpobs in Heqot2. rewrite Heqot2. rewrite bind_vis.
+    gstep. unpriv_ind. admit.
+  - pclearbot. apply simpobs in Heqot1. apply simpobs in Heqot2.
+    rewrite Heqot1. rewrite Heqot2. rewrite bind_vis. rewrite bind_tau.
+    gstep. red. cbn. unpriv_halt. rewrite <- bind_vis. gfinal. left.
+    eapply CIH; eauto.
+  - pclearbot. apply simpobs in Heqot1. apply simpobs in Heqot2.
+    rewrite Heqot1. rewrite Heqot2. rewrite bind_vis. rewrite bind_tau.
+    gstep. red. cbn. unpriv_halt. rewrite <- bind_vis. gfinal. left.
+    eapply CIH; eauto.
+  - pclearbot.  apply simpobs in Heqot1. apply simpobs in Heqot2.
+    rewrite Heqot1. rewrite Heqot2. repeat rewrite bind_vis.
+    gstep. red. cbn. unpriv_halt. red. rewrite <- bind_vis. gfinal. left.
+    eapply CIH; eauto. apply H0.
+  - pclearbot.  apply simpobs in Heqot1. apply simpobs in Heqot2.
+    rewrite Heqot1. rewrite Heqot2. repeat rewrite bind_vis.
+    gstep. red. cbn. unpriv_halt. red. rewrite <- bind_vis. gfinal. left.
+    eapply CIH; eauto. apply H0.Admitted.
+*)
+    
